Implement procedure inlining, factor out boilerplate code in CallElim to BoogieTransform.lean (#232)
*Issue #, if available:*

*Description of changes:*

This pull request
- Implements procedure inlining. It is unverified, but has a few unit
tests; it implements alpha equivalence to check whether the output is
equivalent to the 'answer'
- Factors out the common code that is used between call elimination and
procedure inlining into 'BoogieTransform.lean'. I think this file can be
a nice place for monad, helper functions, etc, for implementing even
more transformations :)


By submitting this pull request, I confirm that you can use, modify,
copy, and redistribute this contribution, under the terms of your
choice.

---------

Co-authored-by: Andrew Wells <130512013+andrewmwells-amazon@users.noreply.github.com>

Strata/Transform/CallElim.lean
@@ -4,198 +4,21 @@
   SPDX-License-Identifier: Apache-2.0 OR MIT
 -/
 
-import Strata.DDM.Integration.Lean
-import Strata.DDM.Util.Format
-import Strata.Languages.Boogie.Statement
-import Strata.Languages.Boogie.Verifier
-import Strata.Languages.Boogie.Boogie
-import Strata.Languages.Boogie.OldExpressions
-import Strata.Languages.Boogie.ProgramWF
-import Strata.DL.Util.ListUtils
-import Strata.Languages.Boogie.BoogieGen
-import Strata.DL.Util.LabelGen
+import Strata.Transform.BoogieTransform
 
 /-! # Call Elimination Transformation -/
 
 namespace Boogie
 namespace CallElim
 
-open LabelGen
-
-def oldVarPrefix (id : String) : String := s!"old_{id}"
-def tmpVarPrefix (id : String) : String := s!"tmp_{id}"
-
-def createHavoc (ident : Expression.Ident)
-  : Statement := Statement.havoc ident
-
-def createHavocs (ident : List Expression.Ident)
-  : List Statement := ident.map createHavoc
-
-def createFvar (ident : Expression.Ident)
-  : Expression.Expr
-  := Lambda.LExpr.fvar ((): ExpressionMetadata) ident none
-
-def createFvars (ident : List Expression.Ident)
-  : List Expression.Expr
-  := ident.map createFvar
-
-def genIdent (ident : Expression.Ident) (pf : String → String)
-  : BoogieGenM Expression.Ident :=
-    BoogieGenState.gen (pf ident.name)
-
-/--
-Generate identifiers in the form of arg_... that can be used to reduce argument expressions to temporary variables.
--/
-def genArgExprIdent (_ : Expression.Expr)
-  : BoogieGenM Expression.Ident :=
-    genIdent "arg" tmpVarPrefix
-
-def genArgExprIdents (exprs : List Expression.Expr)
-  : BoogieGenM (List Expression.Ident)
-  := List.mapM genArgExprIdent exprs
-
-/--
-Retrieves a fresh identifier from the counter generator the given identifier "ident" within old(...), or retrieve an existing one from the exprMap
-Assumes that ident contains no duplicates
--/
-def genOutExprIdent (ident : Expression.Ident)
-  : BoogieGenM Expression.Ident :=
-    genIdent ident tmpVarPrefix
-
-def genOutExprIdents (idents : List Expression.Ident)
-  : BoogieGenM (List Expression.Ident)
-  := List.mapM genOutExprIdent idents
-
-/--
-Retrieves a fresh identifier from the counter generator the given identifier "ident" within old(...), or retrieve an existing one from the exprMap
-Assumes that ident contains no duplicates
--/
-def genOldExprIdent (ident : Expression.Ident)
-  : BoogieGenM Expression.Ident :=
-    genIdent ident oldVarPrefix
-
-def genOldExprIdents (idents : List Expression.Ident)
-  : BoogieGenM (List Expression.Ident)
-  := List.mapM genOldExprIdent idents
-
-/-- Checks whether a variable `ident` can be found in program `p` -/
-def isGlobalVar (p : Program) (ident : Expression.Ident) : Bool :=
-  (p.find? .var ident).isSome
-
-abbrev Err := String
-
-abbrev CallElimM := ExceptT Err BoogieGenM
-
-def getIdentTy? (p : Program) (id : Expression.Ident) := p.getVarTy? id
-
-def getIdentTy! (p : Program) (id : Expression.Ident)
-  : CallElimM (Expression.Ty) := do
-  match getIdentTy? p id with
-  | none => throw s!"failed to find type for {Std.format id}"
-  | some ty => return ty
-
-def getIdentTys! (p : Program) (ids : List Expression.Ident)
-  : CallElimM (List Expression.Ty) := do
-  match ids with
-  | [] => return []
-  | id :: rest =>
-    let ty ← getIdentTy! p id
-    return ty :: (← getIdentTys! p rest)
-
-/--
-returned list has the shape
-((generated_name, ty), original_expr)
--/
-def genArgExprIdentsTrip
-  (inputs : @Lambda.LTySignature Visibility)
-  (args : List Expression.Expr)
-  : CallElimM (List ((Expression.Ident × Lambda.LTy) × Expression.Expr))
-  := do
-  if inputs.length ≠ args.length then throw "input length and args length mismatch"
-  else let gen_idents ← genArgExprIdents args
-       return (gen_idents.zip inputs.unzip.2).zip args
-
-/--
-returned list has the shape
-`((generated_name, ty), original_name)`
--/
-def genOutExprIdentsTrip
-  (outputs : @Lambda.LTySignature Visibility)
-  (lhs : List Expression.Ident)
-  : CallElimM (List ((Expression.Ident × Expression.Ty) × Expression.Ident)) := do
-  if outputs.length ≠ lhs.length then throw "output length and lhs length mismatch"
-  else let gen_idents ← genOutExprIdents lhs
-       return (gen_idents.zip outputs.unzip.2).zip lhs
-
-/--
-returned list has the shape
-`((generated_name, ty), original_name)`
--/
-def genOldExprIdentsTrip
-  (p : Program)
-  (ids : List Expression.Ident)
-  : CallElimM (List ((Expression.Ident × Expression.Ty) × Expression.Ident)) := do
-  let gen_idents ← genOldExprIdents ids
-  let tys ← getIdentTys! p ids
-  return (gen_idents.zip tys).zip ids
-
-/--
-Generate an init statement with rhs as expression
--/
-def createInit (trip : (Expression.Ident × Expression.Ty) × Expression.Expr)
-  : Statement :=
-  match trip with
-  | ((v', ty), e) => Statement.init v' ty e
-
-def createInits (trips : List ((Expression.Ident × Expression.Ty) × Expression.Expr))
-  : List Statement :=
-  trips.map createInit
-
-/--
-Generate an init statement with rhs as a free variable reference
--/
-def createInitVar (trip : (Expression.Ident × Expression.Ty) × Expression.Ident)
-  : Statement :=
-  match trip with
-  | ((v', ty), v) => Statement.init v' ty (Lambda.LExpr.fvar () v none)
-
-def createInitVars (trips : List ((Expression.Ident × Expression.Ty) × Expression.Ident))
-  : List Statement :=
-  trips.map createInitVar
-
-/-- turns a list of preconditions into assumes with substitution -/
-def createAsserts
-    (pres : List Expression.Expr)
-    (subst : Map Expression.Ident Expression.Expr)
-    : List Statement
-    := pres |> List.mapIdx
-                (λ i pred ↦
-                    Statement.assert s!"assert_{i}" (Lambda.LExpr.substFvars pred subst))
-
-/-- turns a list of preconditions into assumes with substitution -/
-def createAssumes
-    (posts : List Expression.Expr)
-    (subst : Map Expression.Ident Expression.Expr)
-    : List Statement
-    := posts |> List.mapIdx
-                  (λ i pred ↦
-                      Statement.assume s!"assume_{i}" (Lambda.LExpr.substFvars pred subst))
-
-/--
-Generate the substitution pairs needed for the body of the procedure
--/
-def createOldVarsSubst
-  (trips : List ((Expression.Ident × Expression.Ty) × Expression.Ident))
-  : Map Expression.Ident Expression.Expr :=
-    trips.map go where go
-    | ((v', _), v) => (v, createFvar v')
+open Boogie.Transform
 
 /--
 The main call elimination transformation algorithm on a single statement.
-The returned result is a sequence of statements if the
+The returned result is a sequence of statements
 -/
 def callElimStmt (st: Statement) (p : Program)
-  : CallElimM (List Statement) := do
+  : BoogieTransformM (List Statement) := do
     match st with
       | .call lhs procName args _ =>
 
@@ -212,12 +35,10 @@ def callElimStmt (st: Statement) (p : Program)
         let oldVars := oldVars.filter (isGlobalVar p)
 
         let genArgTrips := genArgExprIdentsTrip (Lambda.LMonoTySignature.toTrivialLTy proc.header.inputs) args
-
         let argTrips
             : List ((Expression.Ident × Expression.Ty) × Expression.Expr)
             ← genArgTrips
 
-        -- Monadic operation, generate var mapping for each unique oldVars.
         let genOutTrips := genOutExprIdentsTrip (Lambda.LMonoTySignature.toTrivialLTy proc.header.outputs) lhs
         let outTrips
             : List ((Expression.Ident × Expression.Ty) × Expression.Ident)
@@ -264,43 +85,16 @@ def callElimStmt (st: Statement) (p : Program)
         return argInit ++ outInit ++ oldInit ++ asserts ++ havocs ++ assumes
       | _ => return [ st ]
 
-def callElimStmts (ss: List Statement) (prog : Program)
-  : CallElimM (List Statement) := do match ss with
-    | [] => return []
-    | s :: ss =>
-      let s' := (callElimStmt s prog)
-      let ss' := (callElimStmts ss prog)
-      return (← s') ++ (← ss')
+def callElimStmts (ss: List Statement) (prog : Program) :=
+  runStmts callElimStmt ss prog
 
-def callElimL (dcls : List Decl) (prog : Program)
-  : CallElimM (List Decl) :=
-  match dcls with
-  | [] => return []
-  | d :: ds =>
-    match d with
-    | .proc p =>
-      return Decl.proc { p with body := ← (callElimStmts p.body prog ) } :: (← (callElimL ds prog))
-    | _       => return d :: (← (callElimL ds prog))
+def callElimL (dcls : List Decl) (prog : Program) :=
+  runProcedures callElimStmt dcls prog
 
 /-- Call Elimination for an entire program by walking through all procedure
 bodies -/
-def callElim' (p : Program) : CallElimM Program := return { decls := (← (callElimL p.decls p)) }
-
-@[simp]
-def runCallElimWith' {α : Type} (p : α) (f : α → CallElimM β) (s : BoogieGenState):
-  Except Err β × BoogieGenState :=
-  (StateT.run (f p) s)
-
-@[simp]
-def runCallElimWith {α : Type} (p : α) (f : α → CallElimM β) (s : BoogieGenState):
-  Except Err β :=
-  (runCallElimWith' p f s).fst
-
-/-- run call elimination with an empty counter state (e.g. starting from 0) -/
-@[simp]
-def runCallElim {α : Type} (p : α) (f : α → CallElimM β):
-  Except Err β :=
-  runCallElimWith p f .emp
+def callElim' (p : Program) : BoogieTransformM Program :=
+  runProgram callElimStmt p
 
 end CallElim
 end Boogie
