Strata/Transform/BoogieTransform.lean
@@ -1,0 +1,234 @@
+/-
+  Copyright Strata Contributors
+
+  SPDX-License-Identifier: Apache-2.0 OR MIT
+-/
+
+import Strata.Languages.Boogie.Statement
+import Strata.Languages.Boogie.Boogie
+import Strata.Languages.Boogie.BoogieGen
+import Strata.DL.Util.LabelGen
+
+/-! # Utility functions for program transformation in Boogie -/
+
+namespace Boogie
+namespace Transform
+
+open LabelGen
+
+def oldVarPrefix (id : String) : String := s!"old_{id}"
+def tmpVarPrefix (id : String) : String := s!"tmp_{id}"
+
+def createHavoc (ident : Expression.Ident)
+  : Statement := Statement.havoc ident
+
+def createHavocs (ident : List Expression.Ident)
+  : List Statement := ident.map createHavoc
+
+def createFvar (ident : Expression.Ident)
+  : Expression.Expr
+  := Lambda.LExpr.fvar ((): ExpressionMetadata) ident none
+
+def createFvars (ident : List Expression.Ident)
+  : List Expression.Expr
+  := ident.map createFvar
+
+def genIdent (ident : Expression.Ident) (pf : String → String)
+  : BoogieGenM Expression.Ident :=
+    BoogieGenState.gen (pf ident.name)
+
+/--
+Generate identifiers in the form of arg_... that can be used to reduce argument expressions to temporary variables.
+-/
+def genArgExprIdent
+  : BoogieGenM Expression.Ident :=
+    genIdent "arg" tmpVarPrefix
+
+def genArgExprIdents (n:Nat)
+  : BoogieGenM (List Expression.Ident) :=
+  List.mapM (fun _ => genArgExprIdent) (List.replicate n ())
+
+/--
+Retrieves a fresh identifier from the counter generator the given identifier "ident" within old(...), or retrieve an existing one from the exprMap
+Assumes that ident contains no duplicates
+-/
+def genOutExprIdent (ident : Expression.Ident)
+  : BoogieGenM Expression.Ident :=
+    genIdent ident tmpVarPrefix
+
+def genOutExprIdents (idents : List Expression.Ident)
+  : BoogieGenM (List Expression.Ident)
+  := List.mapM genOutExprIdent idents
+
+/--
+Retrieves a fresh identifier from the counter generator the given identifier "ident" within old(...), or retrieve an existing one from the exprMap
+Assumes that ident contains no duplicates
+-/
+def genOldExprIdent (ident : Expression.Ident)
+  : BoogieGenM Expression.Ident :=
+    genIdent ident oldVarPrefix
+
+def genOldExprIdents (idents : List Expression.Ident)
+  : BoogieGenM (List Expression.Ident)
+  := List.mapM genOldExprIdent idents
+
+/-- Checks whether a variable `ident` can be found in program `p` -/
+def isGlobalVar (p : Program) (ident : Expression.Ident) : Bool :=
+  (p.find? .var ident).isSome
+
+abbrev Err := String
+
+abbrev BoogieTransformM := ExceptT Err BoogieGenM
+
+def getIdentTy? (p : Program) (id : Expression.Ident) := p.getVarTy? id
+
+def getIdentTy! (p : Program) (id : Expression.Ident)
+  : BoogieTransformM (Expression.Ty) := do
+  match getIdentTy? p id with
+  | none => throw s!"failed to find type for {Std.format id}"
+  | some ty => return ty
+
+def getIdentTys! (p : Program) (ids : List Expression.Ident)
+  : BoogieTransformM (List Expression.Ty) := do
+  match ids with
+  | [] => return []
+  | id :: rest =>
+    let ty ← getIdentTy! p id
+    return ty :: (← getIdentTys! p rest)
+
+/--
+returned list has the shape
+((generated_name, ty), original_expr)
+Only types of the 'inputs' parameter are used
+-/
+def genArgExprIdentsTrip
+  (inputs : @Lambda.LTySignature Visibility)
+  (args : List Expression.Expr)
+  : BoogieTransformM (List ((Expression.Ident × Lambda.LTy) × Expression.Expr))
+  := do
+  if inputs.length ≠ args.length then throw "input length and args length mismatch"
+  else let gen_idents ← genArgExprIdents args.length
+       return (gen_idents.zip inputs.unzip.2).zip args
+
+/--
+returned list has the shape
+`((generated_name, ty), original_name)`
+Only types of the 'outputs' parameter are used.
+-/
+def genOutExprIdentsTrip
+  (outputs : @Lambda.LTySignature Visibility)
+  (lhs : List Expression.Ident)
+  : BoogieTransformM (List ((Expression.Ident × Expression.Ty) × Expression.Ident)) := do
+  if outputs.length ≠ lhs.length then throw "output length and lhs length mismatch"
+  else let gen_idents ← genOutExprIdents lhs
+       return (gen_idents.zip outputs.unzip.2).zip lhs
+
+/--
+returned list has the shape
+`((generated_name, ty), original_name)`
+-/
+def genOldExprIdentsTrip
+  (p : Program)
+  (ids : List Expression.Ident)
+  : BoogieTransformM (List ((Expression.Ident × Expression.Ty) × Expression.Ident)) := do
+  let gen_idents ← genOldExprIdents ids
+  let tys ← getIdentTys! p ids
+  return (gen_idents.zip tys).zip ids
+
+/--
+Generate an init statement with rhs as expression
+-/
+def createInit (trip : (Expression.Ident × Expression.Ty) × Expression.Expr)
+  : Statement :=
+  match trip with
+  | ((v', ty), e) => Statement.init v' ty e
+
+def createInits (trips : List ((Expression.Ident × Expression.Ty) × Expression.Expr))
+  : List Statement :=
+  trips.map createInit
+
+/--
+Generate an init statement with rhs as a free variable reference
+-/
+def createInitVar (trip : (Expression.Ident × Expression.Ty) × Expression.Ident)
+  : Statement :=
+  match trip with
+  | ((v', ty), v) => Statement.init v' ty (Lambda.LExpr.fvar () v none)
+
+def createInitVars (trips : List ((Expression.Ident × Expression.Ty) × Expression.Ident))
+  : List Statement :=
+  trips.map createInitVar
+
+/-- turns a list of preconditions into assumes with substitution -/
+def createAsserts
+    (pres : List Expression.Expr)
+    (subst : Map Expression.Ident Expression.Expr)
+    : List Statement
+    := pres |> List.mapIdx
+                (λ i pred ↦
+                    Statement.assert s!"assert_{i}" (Lambda.LExpr.substFvars pred subst))
+
+/-- turns a list of preconditions into assumes with substitution -/
+def createAssumes
+    (posts : List Expression.Expr)
+    (subst : Map Expression.Ident Expression.Expr)
+    : List Statement
+    := posts |> List.mapIdx
+                  (λ i pred ↦
+                      Statement.assume s!"assume_{i}" (Lambda.LExpr.substFvars pred subst))
+
+/--
+Generate the substitution pairs needed for the body of the procedure
+-/
+def createOldVarsSubst
+  (trips : List ((Expression.Ident × Expression.Ty) × Expression.Ident))
+  : Map Expression.Ident Expression.Expr :=
+    trips.map go where go
+    | ((v', _), v) => (v, createFvar v')
+
+
+
+/- Generic runner functions -/
+
+def runStmts (f : Statement → Program → BoogieTransformM (List Statement))
+    (ss : List Statement) (inputProg : Program)
+    : BoogieTransformM (List Statement) := do
+  match ss with
+  | [] => return []
+  | s :: ss =>
+    let s' := (f s inputProg)
+    let ss' := (runStmts f ss inputProg)
+    return (← s') ++ (← ss')
+
+def runProcedures (f : Statement → Program → BoogieTransformM (List Statement))
+    (dcls : List Decl) (inputProg : Program)
+    : BoogieTransformM (List Decl) := do
+  match dcls with
+  | [] => return []
+  | d :: ds =>
+    match d with
+    | .proc p =>
+      return Decl.proc { p with body := ← (runStmts f p.body inputProg ) } ::
+        (← (runProcedures f ds inputProg))
+    | _ => return d :: (← (runProcedures f ds inputProg))
+
+def runProgram (f : Statement → Program → BoogieTransformM (List Statement))
+    (p : Program) : BoogieTransformM Program := do
+  let newDecls ← runProcedures f p.decls p
+  return { decls := newDecls }
+
+
+@[simp]
+def runWith {α : Type} (p : α) (f : α → BoogieTransformM β)
+    (s : BoogieGenState):
+  Except Err β × BoogieGenState :=
+  (StateT.run (f p) s)
+
+@[simp]
+def run {α : Type} (p : α) (f : α → BoogieTransformM β)
+      (s : BoogieGenState := .emp):
+  Except Err β :=
+  (runWith p f s).fst
+
+end Transform
+end Boogie
