Strata/Transform/ProcedureInlining.lean
@@ -1,0 +1,260 @@
+/-
+  Copyright Strata Contributors
+
+  SPDX-License-Identifier: Apache-2.0 OR MIT
+-/
+
+import Strata.DL.Util.LabelGen
+import Strata.DL.Util.ListUtils
+import Strata.Languages.Boogie.Boogie
+import Strata.Languages.Boogie.BoogieGen
+import Strata.Languages.Boogie.ProgramWF
+import Strata.Languages.Boogie.Statement
+import Strata.Transform.BoogieTransform
+
+/-! # Procedure Inlining Transformation -/
+
+namespace Boogie
+namespace ProcedureInlining
+
+open Transform
+
+mutual
+partial def Block.substFvar (b : Block) (fr:Expression.Ident)
+      (to:Expression.Expr) : Block :=
+  { b with ss := List.map (fun s => Statement.substFvar s fr to) b.ss }
+
+partial def Statement.substFvar (s : Boogie.Statement)
+      (fr:Expression.Ident)
+      (to:Expression.Expr) : Statement :=
+  match s with
+  | .init lhs ty rhs metadata =>
+    .init lhs ty (Lambda.LExpr.substFvar rhs fr to) metadata
+  | .set lhs rhs metadata =>
+    .set lhs (Lambda.LExpr.substFvar rhs fr to) metadata
+  | .havoc _ _ => s
+  | .assert lbl b metadata =>
+    .assert lbl (Lambda.LExpr.substFvar b fr to) metadata
+  | .assume lbl b metadata =>
+    .assume lbl (Lambda.LExpr.substFvar b fr to) metadata
+  | .call lhs pname args metadata =>
+    .call lhs pname (List.map (Lambda.LExpr.substFvar · fr to) args) metadata
+
+  | .block lbl b metadata =>
+    .block lbl (Block.substFvar b fr to) metadata
+  | .ite cond thenb elseb metadata =>
+    .ite (Lambda.LExpr.substFvar cond fr to) (Block.substFvar thenb fr to)
+          (Block.substFvar elseb fr to) metadata
+  | .loop guard measure invariant body metadata =>
+    .loop (Lambda.LExpr.substFvar guard fr to)
+          (Option.map (Lambda.LExpr.substFvar · fr to) measure)
+          (Option.map (Lambda.LExpr.substFvar · fr to) invariant)
+          (Block.substFvar body fr to)
+          metadata
+  | .goto _ _ => s
+end
+
+mutual
+partial def Block.renameLhs (b : Block) (fr: Lambda.Identifier Visibility) (to: Lambda.Identifier Visibility) : Block :=
+  { b with ss := List.map (fun s => Statement.renameLhs s fr to) b.ss }
+
+partial def Statement.renameLhs (s : Boogie.Statement) (fr: Lambda.Identifier Visibility) (to: Lambda.Identifier Visibility)
+    : Statement :=
+  match s with
+  | .init lhs ty rhs metadata =>
+    .init (if lhs.name == fr then to else lhs) ty rhs metadata
+  | .set lhs rhs metadata =>
+    .set (if lhs.name == fr then to else lhs) rhs metadata
+  | .call lhs pname args metadata =>
+    .call (lhs.map (fun l =>
+      if l.name == fr  then to else l)) pname args metadata
+  | .block lbl b metadata =>
+    .block lbl (Block.renameLhs b fr to) metadata
+  | .ite x thenb elseb m =>
+    .ite x (Block.renameLhs thenb fr to) (Block.renameLhs elseb fr to) m
+  | .loop m g i b md =>
+    .loop m g i (Block.renameLhs b fr to) md
+  | .havoc l md => .havoc (if l.name == fr then to else l) md
+  | .assert _ _ _ | .assume _ _ _
+  | .goto _ _ => s
+end
+
+-- Unlike Stmt.hasLabel, this gathers labels in assert and assume as well.
+mutual
+partial def Block.labels (b : Block): List String :=
+  List.flatMap (fun s => Statement.labels s) b.ss
+
+-- Assume and Assert's labels have special meanings, so they must not be
+-- mangled during procedure inlining.
+partial def Statement.labels (s : Boogie.Statement) : List String :=
+  match s with
+  | .block lbl b _ => lbl :: (Block.labels b)
+  | .ite _ thenb elseb _ => (Block.labels thenb) ++ (Block.labels elseb)
+  | .loop _ _ _ body _ => Block.labels body
+  | .assume lbl _ _ => [lbl]
+  | .assert lbl _ _ => [lbl]
+  | _ => []
+end
+
+mutual
+partial def Block.replaceLabels (b : Block) (map:Map String String)
+    : Block :=
+   { b with ss := b.ss.map (fun s => Statement.replaceLabels s map) }
+
+partial def Statement.replaceLabels
+    (s : Boogie.Statement) (map:Map String String) : Boogie.Statement :=
+  let app (s:String) :=
+    match Map.find? map s with
+    | .none => s
+    | .some s' => s'
+  match s with
+  | .block lbl b m => .block (app lbl) (Block.replaceLabels b map) m
+  | .goto lbl m => .goto (app lbl) m
+  | .ite cond thenb elseb _ =>
+    .ite cond (Block.replaceLabels thenb map) (Block.replaceLabels elseb map)
+  | .loop g measure inv body m =>
+    .loop g measure inv (Block.replaceLabels body map) m
+  | .assume lbl e m => .assume (app lbl) e m
+  | .assert lbl e m => .assert (app lbl) e m
+  | _ => s
+end
+
+
+private def genOldToFreshIdMappings (old_vars : List Expression.Ident)
+    (prev_map : Map Expression.Ident Expression.Ident) (prefix_ : String)
+    : BoogieTransformM (Map Expression.Ident Expression.Ident) := do
+  let prev_map <- old_vars.foldlM
+    (fun var_map id => do
+      let new_name <- genIdent id (fun s => prefix_ ++ "_" ++ s)
+      return var_map.insert id new_name)
+    prev_map
+  return prev_map
+
+private def renameAllLocalNames (c:Procedure)
+    : BoogieTransformM (Procedure × Map Expression.Ident Expression.Ident) := do
+  let var_map: Map Expression.Ident Expression.Ident := []
+  let proc_name := c.header.name.name
+
+  -- Make a map for renaming local variables
+  let lhs_vars := List.flatMap (fun (s:Statement) => s.definedVars) c.body
+  let lhs_vars := lhs_vars ++ c.header.inputs.unzip.fst ++
+                  c.header.outputs.unzip.fst
+  let var_map <- genOldToFreshIdMappings lhs_vars var_map proc_name
+
+  -- Make a map for renaming label names
+  let labels := List.flatMap (fun s => Statement.labels s) c.body
+  -- Reuse genOldToFreshIdMappings by introducing dummy data to Identifier
+  let label_ids:List Expression.Ident := labels.map
+      (fun s => { name:=s, metadata := Visibility.temp })
+  let label_map_id <- genOldToFreshIdMappings label_ids [] proc_name
+  let label_map := label_map_id.map (fun (id1,id2) => (id1.name, id2.name))
+
+  -- Do substitution
+  let new_body := List.map (fun (s0:Statement) =>
+    var_map.foldl (fun (s:Statement) (old_id,new_id) =>
+        let s := Statement.substFvar s old_id (.fvar () new_id .none)
+        let s := Statement.renameLhs s old_id new_id
+        Statement.replaceLabels s label_map)
+      s0) c.body
+  let new_header := { c.header with
+    inputs := c.header.inputs.map (fun (id,ty) =>
+      match var_map.find? id with
+      | .some id' => (id',ty)
+      | .none => panic! "unreachable"),
+    outputs := c.header.outputs.map (fun (id,ty) =>
+      match var_map.find? id with
+      | .some id' => (id',ty)
+      | .none => panic! "unreachable")
+    }
+  return ({ c with body := new_body, header := new_header }, var_map)
+
+
+/-
+Procedure Inlining.
+
+If st is a call statement, inline the contents of the callee procedure.
+To avoid conflicts between duplicated variable names in caller and callee,
+every variables in callee are renamed.
+This function does not update the specification because inlineCallStmt will not
+use the specification. This will have to change if Strata also wants to support
+the reachability query.
+-/
+def inlineCallStmt (st: Statement) (p : Program)
+  : BoogieTransformM (List Statement) :=
+    open Lambda in do
+    match st with
+      | .call lhs procName args _ =>
+
+        let some proc := Program.Procedure.find? p procName
+          | throw s!"Procedure {procName} not found in program"
+
+        -- Create a copy of the procedure that has all input/output/local vars
+        -- replaced with fresh ones
+        let (proc,var_map) <- renameAllLocalNames proc
+
+        let sigOutputs := LMonoTySignature.toTrivialLTy proc.header.outputs
+        let sigInputs := LMonoTySignature.toTrivialLTy proc.header.inputs
+
+        -- Stuffs for the call statement:
+        --   call x1,x2, .. = f(v1,v2,...)
+        --   where 'procedure f(in1,in2,..) outputs(out1,out2,..)'
+        -- Insert
+        --   init in1 : ty := v1     --- inputInit
+        --   init in2 : ty := v2
+        --   init out1 : ty := <placeholder> --- outputInit
+        --   init out2 : ty := <placeholder>
+        --   ... (f body)
+        --   set x1 := out1    --- outputSetStmts
+        --   set x2 := out2
+        -- `init outN` is not necessary because calls are only allowed to use
+        -- already declared variables (per Boogie.typeCheck)
+
+        -- Create a fresh var statement for each LHS
+        let outputTrips ← genOutExprIdentsTrip sigOutputs sigOutputs.unzip.fst
+        let outputInit := createInitVars
+          (outputTrips.map (fun ((tmpvar,ty),orgvar) => ((orgvar,ty),tmpvar)))
+        -- Create a var statement for each procedure input arguments.
+        -- The input parameter expression is assigned to these new vars.
+        --let inputTrips ← genArgExprIdentsTrip sigInputs args
+        let inputInit := createInits (sigInputs.zip args)
+        -- Assign the output variables in the signature to the actual output
+        -- variables used in the callee.
+        let outputSetStmts :=
+          let out_vars := sigOutputs.unzip.fst
+          let out_vars := out_vars.map
+              (fun id => match var_map.find? id with
+                  | .none => id | .some x => x)
+          let outs_lhs_and_sig := List.zip lhs out_vars
+          List.map
+            (fun (lhs_var,out_var) =>
+              Statement.set lhs_var (.fvar () out_var (.none)))
+            outs_lhs_and_sig
+
+        let stmts:List (Imperative.Stmt Boogie.Expression Boogie.Command)
+          := inputInit ++ outputInit ++ proc.body ++ outputSetStmts
+        let new_blk := Imperative.Block.mk stmts
+
+        return [.block (procName ++ "$inlined") new_blk]
+      | _ => return [st]
+
+def inlineCallStmts (ss: List Statement) (prog : Program)
+  : BoogieTransformM (List Statement) := do match ss with
+    | [] => return []
+    | s :: ss =>
+      let s' := (inlineCallStmt s prog)
+      let ss' := (inlineCallStmts ss prog)
+      return (← s') ++ (← ss')
+
+def inlineCallL (dcls : List Decl) (prog : Program)
+  : BoogieTransformM (List Decl) :=
+  match dcls with
+  | [] => return []
+  | d :: ds =>
+    match d with
+    | .proc p =>
+      return Decl.proc { p with body := ← (inlineCallStmts p.body prog ) } ::
+        (← (inlineCallL ds prog))
+    | _       => return d :: (← (inlineCallL ds prog))
+
+end ProcedureInlining
+end Boogie
