StrataTest/Transform/DetToNondet.lean
@@ -1,0 +1,40 @@
+/-
+  Copyright Strata Contributors
+
+  SPDX-License-Identifier: Apache-2.0 OR MIT
+-/
+
+import Strata.Transform.DetToNondet
+import Strata.Languages.Boogie.StatementSemantics
+import Strata.Languages.Boogie.ProgramType
+import Strata.Languages.Boogie.ProgramWF
+import Strata.DL.Lambda.IntBoolFactory
+
+open Boogie
+
+/-! ## Deterministic-to-Nondeterministic Examples -/
+section NondetExamples
+
+open Imperative
+
+def NondetTest1 : Stmt Expression (Cmd Expression) :=
+  .ite (Boogie.true) {ss :=
+    [.cmd $ .havoc "x" ]
+    } {ss :=
+    [.cmd $ .havoc "y" ]
+    }
+
+def NondetTest1Ans : NondetStmt Expression (Cmd Expression) :=
+  .choice
+    (.seq (.cmd (.assume "true_cond" Boogie.true)) (.seq (.cmd $ .havoc "x") (.assume "skip" Imperative.HasBool.tt)))
+    (.seq (.cmd (.assume "false_cond" Boogie.false)) (.seq (.cmd $ .havoc "y") (.assume "skip" Imperative.HasBool.tt)))
+
+
+-- #eval toString $ Std.format (StmtToNondetStmt NondetTest1)
+-- #eval toString $ Std.format NondetTest1Ans
+
+/-- info: true -/
+#guard_msgs in
+#eval (toString $ Std.format (StmtToNondetStmt NondetTest1)) == (toString $ Std.format NondetTest1Ans)
+
+end NondetExamples
