StrataTest/Transform/ProcedureInlining.lean
@@ -1,0 +1,340 @@
+/-
+  Copyright Strata Contributors
+
+  SPDX-License-Identifier: Apache-2.0 OR MIT
+-/
+
+import Strata.DDM.Integration.Lean
+import Strata.DDM.Util.Format
+import Strata.Languages.Boogie.Boogie
+import Strata.Languages.Boogie.DDMTransform.Translate
+import Strata.Languages.Boogie.StatementSemantics
+import Strata.Languages.Boogie.ProgramType
+import Strata.Languages.Boogie.ProgramWF
+import Strata.Transform.BoogieTransform
+import Strata.Transform.ProcedureInlining
+
+open Boogie
+open Boogie.Transform
+open ProcedureInlining
+open Strata
+open Std
+
+/-! ## Procedure Inlining Examples -/
+
+section ProcedureInliningExamples
+
+
+-- Alpha equivalence of procedures for testing!
+
+
+structure IdMap where
+  vars: Map String String
+  labels: Map String String
+
+private def IdMap.updateVars (map:IdMap) (newmap: List (String × String))
+  : Except Format IdMap := do
+  let newvars ← newmap.foldlM (fun m ((oldid,newid):String × String) =>
+    match Map.find? m oldid with
+    | .some x => .error  (f!"Has duplicated definition of var " ++ oldid ++
+        "(previously mapped to " ++ x ++ ")")
+    | .none => return (m.insert oldid newid))
+    map.vars
+  return { map with vars := newvars }
+
+private def IdMap.updateLabel (map:IdMap) (frlbl:String) (tolbl:String)
+  : Except Format IdMap := do
+  match Map.find? map.labels frlbl with
+  | .none =>
+    return { map with labels := Map.insert map.labels frlbl tolbl }
+  | .some x =>
+    if x == tolbl then return map
+    else .error ("Label " ++ frlbl ++ " is already mapped to " ++ x ++
+      " but tried to map to " ++ tolbl)
+
+private def IdMap.varMapsTo (map:IdMap) (fr:String) (to:String): Bool :=
+  match Map.find? map.vars fr with
+  | .none => false
+  | .some x => x == to
+
+private def IdMap.lblMapsTo (map:IdMap) (fr:String) (to:String): Bool :=
+  match Map.find? map.labels fr with
+  | .none => false
+  | .some x => x == to
+
+
+private def substExpr (e1:Expression.Expr) (map:IdMap) :=
+  map.vars.foldl
+    (fun (e:Expression.Expr) ((i1,i2):String × String) =>
+      -- old_id has visibility of temp because the new local variables were
+      -- created by BoogieGenM.
+      let old_id:Expression.Ident := { name := i1, metadata := Visibility.temp }
+      -- new_expr has visibility of unres because that is the default setting
+      -- from DDM parsed program, and the substituted program is supposed to be
+      -- equivalent to the answer program translated from DDM
+      let new_expr:Expression.Expr := .fvar ()
+          { name := i2, metadata := Visibility.unres } .none
+      e.substFvar old_id new_expr)
+    e1
+
+private def alphaEquivExprs (e1 e2: Expression.Expr) (map:IdMap)
+    : Bool :=
+  (substExpr e1 map).eraseTypes == e2.eraseTypes
+
+private def alphaEquivExprsOpt (e1 e2: Option Expression.Expr) (map:IdMap)
+    : Except Format Bool :=
+  match e1,e2 with
+  | .some e1, .some e2 =>
+    return alphaEquivExprs e1 e2 map
+  | .none, .none =>
+    return .true
+  | _, _ =>
+    .error ".some and .none mismatch"
+
+private def alphaEquivIdents (e1 e2: Expression.Ident) (map:IdMap)
+    : Bool :=
+  (-- Case 1: e1 is created from inliner, e2 was from DDM
+   (e1.metadata == Visibility.temp && e2.metadata == Visibility.unres) ||
+   -- Caes 2: both e1 and e2 are from DDM
+   (e1.metadata == e2.metadata)) &&
+  (match Map.find? map.vars e1.name with
+    | .some n' => n' == e2.name
+    | .none => e1.name == e2.name)
+
+
+mutual
+
+partial def alphaEquivBlock (b1 b2: Boogie.Block) (map:IdMap)
+    : Except Format IdMap := do
+  let st1 := b1.ss
+  let st2 := b2.ss
+  if st1.length ≠ st2.length then
+    .error "Block lengths do not match"
+  else
+    (st1.zip st2).foldlM
+      (fun (map:IdMap) (st1,st2) => do
+        let newmap ← alphaEquivStatement st1 st2 map
+        return newmap)
+      map
+
+partial def alphaEquivStatement (s1 s2: Boogie.Statement) (map:IdMap)
+    : Except Format IdMap := do
+  let mk_err (s:Format): Except Format IdMap :=
+    .error (f!"{s}\ns1:{s1}\ns2:{s2}\nmap:{map.vars}")
+
+  match (s1,s2) with
+  | (.block lbl1 b1 _, .block lbl2 b2 _) =>
+    -- Since 'goto lbl' can appear before 'lbl' is defined, update the label
+    -- map here
+    let map ← IdMap.updateLabel map lbl1 lbl2
+    alphaEquivBlock b1 b2 map
+
+  | (.ite cond1 thenb1 elseb1 _, .ite cond2 thenb2 elseb2 _) => do
+    if alphaEquivExprs cond1 cond2 map then
+      let map' <- alphaEquivBlock thenb1 thenb2 map
+      let map'' <- alphaEquivBlock elseb1 elseb2 map'
+      return map''
+    else
+      .error "if conditions do not match"
+
+  | (.loop g1 m1 i1 b1 _, .loop g2 m2 i2 b2 _) =>
+    if ¬ alphaEquivExprs g1 g2 map then
+      .error "guard does not match"
+    else if ¬ (← alphaEquivExprsOpt m1 m2 map) then
+      .error "measure does not match"
+    else if ¬ (← alphaEquivExprsOpt i1 i2 map) then
+      .error "invariant does not match"
+    else alphaEquivBlock b1 b2 map
+
+  | (.goto lbl1 _, .goto lbl2 _) =>
+    IdMap.updateLabel map lbl1 lbl2
+
+  | (.cmd c1, .cmd c2) =>
+    match (c1, c2) with
+    | (.call lhs1 procName1 args1 _, .call lhs2 procName2 args2 _) =>
+      if procName1 ≠ procName2 then
+        .error "Procedure name does not match"
+      else if lhs1.length ≠ lhs2.length then
+        .error "Call LHS length does not match"
+      else if ¬ (lhs1.zip lhs2).all
+          (fun (lhs1,lhs2) => alphaEquivIdents lhs1 lhs2 map) then
+        .error "Call LHS name does not map"
+      else if (args1.length ≠ args2.length) then
+        .error "Call args length does not match"
+      else if ¬ (args1.zip args2).all (fun (arg1,arg2) =>
+          ¬ alphaEquivExprs arg1 arg2 map) then
+        .error "Call args do not map"
+      else
+        return map
+    | (.cmd (.init n1 _ _e1 _), .cmd (.init n2 _ _e2 _)) =>
+      -- Omit e1 and e2 check because init may use undeclared free vars
+      -- The updateVars below must be the only place that updates the
+      -- variable name mapping.
+      IdMap.updateVars map [(n1.name,n2.name)]
+    | (.cmd (.set n1 e1 _), .cmd (.set n2 e2 _)) =>
+      if ¬ alphaEquivExprs e1 e2 map then
+        mk_err f!"RHS of sets do not match \
+        \n(subst of e1: {repr (substExpr e1 map)})\n(e2: {repr e2})"
+      else if ¬ alphaEquivIdents n1 n2 map then
+        mk_err "LHS of sets do not match"
+      else
+        return map
+    | (.cmd (.havoc n1 _), .cmd (.havoc n2 _)) =>
+      if ¬ alphaEquivIdents n1 n2 map then
+        mk_err "LHS of havocs do not match"
+      else
+        return map
+    | (.cmd (.assert _ e1 _), .cmd (.assert _ e2 _)) =>
+      if ¬ alphaEquivExprs e1 e2 map then
+        mk_err "Expressions of asserts do not match"
+      else
+        return map
+    | (.cmd (.assume _ e1 _), .cmd (.assume _ e2 _)) =>
+      if ¬ alphaEquivExprs e1 e2 map then
+        mk_err "Expressions of assumes do not match"
+      else
+        return map
+    | (_,_) =>
+      mk_err "Commands do not match"
+
+  | (_,_) => mk_err "Statements do not match"
+
+end
+
+private def alphaEquiv (p1 p2:Boogie.Procedure):Except Format Bool := do
+  if p1.body.length ≠ p2.body.length then
+    dbg_trace f!"p1: {p1}"
+    dbg_trace f!"p2: {p2}"
+    .error (s!"# statements do not match: inlined fn one has {p1.body.length}"
+        ++ s!" whereas the answer has {p2.body.length}")
+  else
+    let newmap:IdMap := IdMap.mk [] []
+    let stmts := (p1.body.zip p2.body)
+    let _ ← List.foldlM (fun (map:IdMap) (s1,s2) =>
+        alphaEquivStatement s1 s2 map)
+      newmap stmts
+    return .true
+
+
+
+def translate (t : Strata.Program) : Boogie.Program :=
+  (TransM.run Inhabited.default (translateProgram t)).fst
+
+def runInlineCall (p : Boogie.Program) : Boogie.Program :=
+  match (runProgram inlineCallStmt p .emp) with
+  | ⟨.ok res, _⟩ => res
+  | ⟨.error e, _⟩ => panic! e
+
+def checkInlining (prog : Boogie.Program) (progAns : Boogie.Program)
+    : Except Format Bool := do
+  let prog' := runInlineCall prog
+  let pp' := prog'.decls.zip progAns.decls
+  pp'.allM (fun (p,p') => do
+    match p,p' with
+    | .proc p, .proc p' =>
+      match alphaEquiv p p' with
+      | .ok _ => return .true
+      | .error msg =>
+        dbg_trace s!"{toString prog'}"
+        dbg_trace s!"{toString progAns}"
+        .error msg
+    | _, _ => .error "?")
+
+
+
+def Test1 :=
+#strata
+program Boogie;
+procedure f(x : bool) returns (y : bool) {
+  havoc x;
+  y := !x;
+};
+
+procedure h() returns () {
+  var b_in : bool;
+  var b_out : bool;
+  call b_out := f(b_in);
+};
+#end
+
+def Test1Ans :=
+#strata
+program Boogie;
+procedure f(x : bool) returns (y : bool) {
+  havoc x;
+  y := !x;
+};
+
+procedure h() returns () {
+  var b_in : bool;
+  var b_out : bool;
+  inlined: {
+    var tmp_arg_0 : bool := b_in;
+    var tmp_arg_1 : bool;
+    havoc tmp_arg_0;
+    tmp_arg_1 := !tmp_arg_0;
+    b_out := tmp_arg_1;
+  }
+};
+
+#end
+
+/-- info: ok: true -/
+#guard_msgs in
+#eval checkInlining (translate Test1) (translate Test1Ans)
+
+def Test2 :=
+#strata
+program Boogie;
+procedure f(x : bool) returns (y : bool) {
+  if (x) {
+    goto end;
+  } else { y := false;
+  }
+  end: {}
+};
+
+procedure h() returns () {
+  var b_in : bool;
+  var b_out : bool;
+  call b_out := f(b_in);
+  end: {}
+};
+#end
+
+def Test2Ans :=
+#strata
+program Boogie;
+procedure f(x : bool) returns (y : bool) {
+  if (x) {
+    goto end;
+  } else { y := false;
+  }
+  end: {}
+};
+
+procedure h() returns () {
+  var b_in : bool;
+  var b_out : bool;
+  inlined: {
+    var f_x : bool := b_in;
+    var f_y : bool;
+    if (f_x) {
+      goto f_end;
+    } else {
+      f_y := false;
+    }
+    f_end: {}
+    b_out := f_y;
+  }
+  end: {}
+};
+
+#end
+
+/-- info: ok: true -/
+#guard_msgs in
+#eval checkInlining (translate Test2) (translate Test2Ans)
+
+
+end ProcedureInliningExamples
